untyped in progress

Fos/Datatypes.lean
@@ -7,57 +7,253 @@ import Fos.Reduce
 namespace Fos
 
 def btrue : Term :=
-  sorry
+  -- λt. λf. t
+  Term.t_abs (Term.t_abs (Term.t_var 1))
 
 def bfalse : Term :=
-  sorry
+  -- λt. λf. f
+  Term.t_abs (Term.t_abs (Term.t_var 0))
 
 def or : Term :=
-  sorry
-
+  -- λb. λc. b tru c
+  Term.t_abs (Term.t_abs (Term.t_app (Term.t_app (Term.t_var 1)
+                                                 btrue)
+                                     (Term.t_var 0)))
 def and : Term :=
-  sorry
-
+  -- λb. λc. b c fls
+  Term.t_abs (Term.t_abs (Term.t_app (Term.t_app (Term.t_var 1)
+                                                 (Term.t_var 0))
+                                     bfalse))
 def not : Term :=
-  sorry
+  -- λb. b fls tru
+  Term.t_abs (Term.t_app (Term.t_app (Term.t_var 0)
+                                     bfalse)
+                         btrue)
 
-theorem boolean_expr_simple :=
+theorem boolean_expr_simple :
+  Term.t_app not
+             (Term.t_app (Term.t_app and
+                                     btrue)
+                         bfalse) ~~>* btrue := by
+  -- This lemma is wrong.
+  --have h0 : ∀ (t : Term), Term.t_app btrue t ~~>* Term.t_abs t := by
+
+  have h1 : ∀ (t : Term), Term.t_app (Term.t_app btrue
+                                                 t)
+                                     bfalse ~~>* t := by
+    intro t
+    simp [btrue]
+
+    apply Relation.ReflTransGen.head
+    apply Reduce.e_appabs
+
+  have h1 : Term.t_app and btrue ~~>* Term.t_abs (Term.t_app (Term.t_app btrue
+                                                                          (Term.t_var 0))
+                                                              bfalse) := by
+    simp [and]
+    apply Relation.ReflTransGen.single
+    apply Reduce.e_appabs
+
+  have h2 : Term.t_app (Term.t_app and
+                                   btrue)
+                       bfalse ~~>* bfalse := by
+    apply Relation.ReflTransGen.trans
+    apply reduce_many_app1 h1
+    simp
+
+    apply Relation.ReflTransGen.head
+    apply Reduce.e_appabs
+    simp [btrue]
+
+    apply Relation.ReflTransGen.head
+    apply Reduce.e_appabs
+    sorry
+
+
   sorry
 
 -- Arithmetic
 
 def iszero :=
-  sorry
-
+  -- λm. m (λx. fls) tru
+  Term.t_abs (Term.t_app (Term.t_app (Term.t_var 0)
+                                     (Term.t_abs bfalse))
+                         btrue)
 theorem iszero_zero : elaborate ({iszero}({zero})) ~~>* btrue := by
-  sorry
+  simp [iszero, zero]
+  -- (λm. m (λx. fls) tru) (λs. λz. z)
+  apply Relation.ReflTransGen.head
+  apply Reduce.e_appabs
+  -- (λs. λz. z) (λx. fls) tru
+  apply Relation.ReflTransGen.head
+  apply Reduce.e_app1
+  apply Reduce.e_appabs
+  -- (λz. z) tru
+  apply Relation.ReflTransGen.head
+  apply Reduce.e_appabs
+  -- tru
+  simp [btrue]
+  apply Relation.ReflTransGen.refl
 
 theorem iszero_succ : elaborate (λ "n" => {iszero}({succ}("n"))) ~~>* elaborate (λ "n" => {bfalse}) := by
-  sorry
+  simp [iszero, succ]
+  -- λn. ( (λm. m (λx. fls) tru) (λn. λs. λz. s (n s z)) )
+  apply Relation.ReflTransGen.head
+  apply Reduce.e_abs
+  apply Reduce.e_appabs
+  -- λn. ( (λn. λs. λz. s (n s z)) (λx. fls) tru)
+  apply Relation.ReflTransGen.head
+  apply Reduce.e_abs
+  apply Reduce.e_app1
+  apply Reduce.e_appabs
 
 -- Fold lists
 
 def flist_nil :=
-  sorry
+  -- λf. λz. z
+  Term.t_abs (Term.t_abs (Term.t_var 0))
 
 def flist_cons :=
-  sorry
-
+  -- λh. λt. λf. λz. f h (t f z)
+  -- A list is encoded as its own fold function.
+  Term.t_abs (Term.t_abs (Term.t_abs (Term.t_abs (
+    Term.t_app (Term.t_app
+        (Term.t_var 1)
+        (Term.t_var 3)
+      )
+      (Term.t_app (Term.t_app
+          (Term.t_var 2)
+          (Term.t_var 1)
+        )
+        (Term.t_var 0)
+      )
+  ))))
 def flist_isnil :=
-  sorry
+  -- λl. l (λh. λt. fls) tru
+  Term.t_abs (Term.t_app (Term.t_app (Term.t_var 0)
+                                     (Term.t_abs (Term.t_abs bfalse)))
+                         btrue)
 
 theorem flist_isnil_nil : elaborate ({flist_isnil}({flist_nil})) ~~>* btrue := by
-  sorry
+  simp [flist_isnil, flist_nil]
+  -- (λl. l (λh. λt. fls) tru) (λf. λz. z)
+  apply Relation.ReflTransGen.head
+  apply Reduce.e_appabs
+  -- (λf. λz. z) (λh. λt. fls) tru
+  apply Relation.ReflTransGen.head
+  apply Reduce.e_app1
+  apply Reduce.e_appabs
+  -- (λz. z) tru
+  apply Relation.ReflTransGen.head
+  apply Reduce.e_appabs
+  -- tru
+  simp [btrue]
+  apply Relation.ReflTransGen.refl
 
 theorem flist_isnil_cons :
   elaborate (λ "h" => λ "t" => {flist_isnil}({flist_cons}("h")("t")))
   ~~>* elaborate (λ "h" => λ "t" => {bfalse}) := by
-  sorry
+  -- λh. λt. flist_isnil (flist_cons h t)
+  simp [flist_isnil, flist_cons]
+  -- λh. λt. (λl. l (λh'. λt'. fls) tru) ( (λh". λt". λf. λz. f h" (t" f z)) h t)
+  apply Relation.ReflTransGen.head
+  apply Reduce.e_abs
+  apply Reduce.e_abs
+  apply Reduce.e_appabs
+  -- λh. λt. ( ( (λh". λt". λf. λz. f h" (t" f z)) h t) (λh'. λt'. fls) tru)
+  apply Relation.ReflTransGen.head
+  apply Reduce.e_abs
+  apply Reduce.e_abs
+  apply Reduce.e_app1
+  apply Reduce.e_app1
+  apply Reduce.e_app1
+  apply Reduce.e_appabs
+  -- λh. λt. ( ( (λt". λf. λz. f h (t" f z)) t) (λh'. λt'. fls) tru)
+  apply Relation.ReflTransGen.head
+  apply Reduce.e_abs
+  apply Reduce.e_abs
+  apply Reduce.e_app1
+  apply Reduce.e_app1
+  apply Reduce.e_appabs
+  -- λh. λt. ( (λf. λz. f h (t f z)) (λh'. λt'. fls) tru)
+  apply Relation.ReflTransGen.head
+  apply Reduce.e_abs
+  apply Reduce.e_abs
+  apply Reduce.e_app1
+  apply Reduce.e_appabs
+  -- λh. λt. ( (λz. (λh'. λt'. fls) h (t (λh'. λt'. fls) z)) tru)
+  apply Relation.ReflTransGen.head
+  apply Reduce.e_abs
+  apply Reduce.e_abs
+  apply Reduce.e_appabs
+  -- λh. λt. ( (λh'. λt'. fls) h (t (λh'. λt'. fls) tru) )
+  apply Relation.ReflTransGen.head
+  apply Reduce.e_abs
+  apply Reduce.e_abs
+  apply Reduce.e_app1
+  apply Reduce.e_appabs
+  -- λh. λt. ( (λt'. fls) (t (λh'. λt'. fls) tru) )
+  apply Relation.ReflTransGen.head
+  apply Reduce.e_abs
+  apply Reduce.e_abs
+  apply Reduce.e_appabs
+  -- λh. λt. fls
+  simp [btrue]
+  apply Relation.ReflTransGen.refl
 
 def flist_head :=
-  sorry
-
+  -- λl. l (λh. λt. h) dummy
+  Term.t_abs (
+    Term.t_app (Term.t_app
+      (Term.t_var 0)
+      (Term.t_abs (Term.t_abs (Term.t_var 1)))
+    )
+    btrue -- Dummy term
+  )
 theorem flist_head_cons : elaborate (λ "h" => λ "t" => {flist_head}({flist_cons}("h")("t"))) ~~>* elaborate (λ "h" => λ "t" => "h") := by
-  sorry
+  -- λh. λt. flist_head (flist_cons h t)
+  simp [flist_head, flist_cons]
+  -- λh. λt. (λl. l (λh'. λt'. h') dummy) ( (λh". λt". λf. λz. f h" (t" f z)) h t)
+  apply Relation.ReflTransGen.head
+  apply Reduce.e_abs
+  apply Reduce.e_abs
+  apply Reduce.e_app2
+  apply Reduce.e_app1
+  apply Reduce.e_appabs
+  -- λh. λt. (λl. l (λh'. λt'. h') dummy) ( (λt". λf. λz. f h (t" f z)) t)
+  apply Relation.ReflTransGen.head
+  apply Reduce.e_abs
+  apply Reduce.e_abs
+  apply Reduce.e_app2
+  apply Reduce.e_appabs
+  -- λh. λt. (λl. l (λh'. λt'. h') dummy) (λf. λz. f h (t f z))
+  apply Relation.ReflTransGen.head
+  apply Reduce.e_abs
+  apply Reduce.e_abs
+  apply Reduce.e_appabs
+  -- λh. λt. ( (λf. λz. f h (t f z)) (λh'. λt'. h') dummy)
+  apply Relation.ReflTransGen.head
+  apply Reduce.e_abs
+  apply Reduce.e_abs
+  apply Reduce.e_app1
+  apply Reduce.e_appabs
+  -- λh. λt. ( (λz. (λh'. λt'. h') h (t (λh'. λt'. h') z)) dummy)
+  apply Relation.ReflTransGen.head
+  apply Reduce.e_abs
+  apply Reduce.e_abs
+  apply Reduce.e_appabs
+  -- λh. λt. ( (λh'. λt'. h') h (t (λh'. λt'. h') dummy) )
+  apply Relation.ReflTransGen.head
+  apply Reduce.e_abs
+  apply Reduce.e_abs
+  apply Reduce.e_app1
+  apply Reduce.e_appabs
+  -- λh. λt. ( (λt'. h) (t (λh'. λt'. h') dummy) )
+  apply Relation.ReflTransGen.head
+  apply Reduce.e_abs
+  apply Reduce.e_abs
+  apply Reduce.e_appabs
+  -- λh. λt. h
+  apply Relation.ReflTransGen.refl
 
 end Fos
