Fos/Syntax.lean
@@ -20,6 +20,7 @@ notation "λ" n " => " t => Syntax.s_lam n t
 notation t1 "(" t2 ")" => Syntax.s_app t1 t2
 notation "{" t "}" => Syntax.s_value t
 
+@[simp]
 def lookupName (n : String) : List String -> Option Nat
 -- Define the lookup function
 | [] => none
