Fos/Term.lean
@@ -13,26 +13,31 @@ def Subst : Type := Nat -> Term
 
 def Rename.comp (f : Rename) (g : Rename) : Rename := fun x => g (f x)
 
+@[simp]
 def Rename.lift (f : Rename) : Rename
 | 0 => 0
 | n+1 => (f n)+1
 
+@[simp]
 def Term.rename (t : Term) (f : Rename) : Term :=
   match t with
   | t_var n => t_var (f n)
   | t_abs t => t_abs (t.rename f.lift)
   | t_app t1 t2 => t_app (t1.rename f) (t2.rename f)
 
+@[simp]
 def Subst.lift (s : Subst) : Subst
 | 0 => .t_var 0
 | n+1 => (s n).rename Nat.succ
 
+@[simp]
 def Term.subst (t : Term) (s : Subst) : Term :=
   match t with
   | t_var n => s n
   | t_abs t => t_abs (t.subst s.lift)
   | t_app t1 t2 => t_app (t1.subst s) (t2.subst s)
 
+@[simp]
 def Subst.subst_zero (t : Term) : Subst
 | 0 => t
 | n+1 => .t_var n
@@ -40,6 +45,7 @@ def Subst.subst_zero (t : Term) : Subst
 /-
 Substitutes the zero-indexed variable with the given term.
 -/
+@[simp]
 def Term.subst_zero (t : Term) (u : Term) : Term :=
   t.subst (Subst.subst_zero u)
 
