README.md
@@ -51,13 +51,13 @@ The definition of `Reduce` should match the rules on the page 55 of the Week 3 s
 
 Open `Datatypes.lean`.
 
-> _Question 6:_ Fill in the definitions for `btrue`, `bfalse`, `or`, and `and`.
+> _~~Question 6~~:_ Fill in the definitions for `btrue`, `bfalse`, `or`, and `and`.
 
 > _Question 7:_ State and prove that `not (and btrue bfalse) ~~>* btrue` (`boolean_expr_simple`)
 
 > _Question 8:_ Define `iszero` and state and prove the expected lemma for it: `iszero zero` reduces to `btrue` (`iszero_zero`), `iszero (succ n)` reduces to `bfalse` (`iszero_succ`).
 
-> _Question 9:_ Define `flist_nil`, `flist_cons` in the style of fold-left lists. Define `flist_isnil` and prove the expected theorems about it: `isnil nil` reduces to `btrue` (`flist_isnil_nil`) and `isnil (cons h t)` reduces to `bfalse` (`flist_isnil_cons`).
+> _~~Question 9~~:_ Define `flist_nil`, `flist_cons` in the style of fold-left lists. Define `flist_isnil` and prove the expected theorems about it: `isnil nil` reduces to `btrue` (`flist_isnil_nil`) and `isnil (cons h t)` reduces to `bfalse` (`flist_isnil_cons`).
 
 > _Optional_: Define `flist_head` and prove the theorem about it: `head (cons h t)` reduces to `h` (`flist_head_cons`).
 
